try some automation

ML_SP_Unify.v
@@ -251,21 +251,26 @@ Qed.
 
 Lemma add_binding_is_subst : forall S x T,
   is_subst S ->
-  disjoint (dom S \u {{x}}) (typ_fv T) ->
+  disjoint (dom S) (typ_fv T) ->
+  x \notin (typ_fv T) ->
   is_subst (compose (x ~ T) S).
 Proof.
   intros.
   unfold compose.
   intro; intros.
-  binds_cases H1.
+  binds_cases H2.
     destruct (binds_map_inv _ _ B) as [b [F B']].
     subst.
     use (H _ _ B').
     simpl in *.
     apply* disjoint_subst.
+    intro y; destruct* (H0 y). destruct* (y == x).
   destruct (binds_single_inv B0); subst.
-  auto.
+  disjoint_solve.
+  destruct* (v == x0).
 Qed.
+
+Hint Resolve add_binding_is_subst.
 
 Lemma typ_subst_disjoint : forall S T,
   is_subst S -> disjoint (dom S) (typ_fv (typ_subst S T)).
@@ -278,6 +283,16 @@ Proof.
     simpl; intro x; destruct* (x == v).
   disjoint_solve.
 Qed.
+
+Lemma typ_subst_res_fresh : forall S T T',
+  is_subst S -> typ_subst S T = T' -> disjoint (dom S) (typ_fv T').
+Proof.
+  intros.
+  use (typ_subst_disjoint T H).
+  rewrite* <- H0.
+Qed.
+
+Hint Resolve typ_subst_disjoint typ_subst_res_fresh.
 
 Lemma binds_add_binding : forall S T0 T1 v x T,
   is_subst S ->
@@ -299,6 +314,8 @@ Proof.
   simpl; disjoint_solve.
 Qed.
 
+Hint Resolve binds_add_binding.
+
 Lemma unify_keep_nv : forall h pairs K K' T S S' t t0 v,
   (forall K S,
     unify h pairs K S = Some (K', S') ->
@@ -319,16 +336,14 @@ Proof.
   case_rewrite (S.mem v (typ_fv T)) R3.
   fold kind in *.
   case_rewrite (get_kind v K) R4.
-  destruct (IHh _ _ H); clear IHh.
-    apply* add_binding_is_subst.
-    simpl.
-    use (typ_subst_disjoint t0 HS). rewrite R2 in H0.
-    disjoint_solve.
-    destruct* (v0 == v). subst*.
-  split*.
-  intros; apply H1.
-  apply* binds_add_binding.
+  destruct* (IHh _ _ H); clear IHh.
 Qed.
+
+Lemma neq_notin_fv : forall v v0,
+  v <> v0 -> v \notin (typ_fv (typ_fvar v0)).
+Proof. simpl*. Qed.
+
+Hint Resolve neq_notin_fv.
 
 Lemma unify_keep : forall h pairs K S K' S',
   unify h pairs K S = Some (K', S') ->
@@ -343,31 +358,23 @@ Proof.
   destruct p.
   case_rewrite (typ_subst S t) R1; case_rewrite (typ_subst S t0) R2.
         destruct (n === n0).
-          apply* (IHh _ _ _ _ _ H).
+          apply* IHh.
         discriminate.
        apply* (@unify_keep_nv h pairs K K' (typ_bvar n)).
        intros. apply* IHh.
       apply* (@unify_keep_nv h pairs K K' (typ_bvar n)).
-      intros. apply* IHh.
+      intros; apply* IHh.
      destruct (v == v0).
-       destruct* (IHh _ _ _ _ _ H).
+       apply* IHh.
      unfold unify_vars in H.
      destruct (unify_kinds (get_kind v K) (get_kind v0 K)) as [[k1 l]|];
        try discriminate.
-     destruct (IHh _ _ _ _ _ H); clear IHh.
-       apply* add_binding_is_subst.
-       simpl.
-       use (typ_subst_disjoint t0 H0). rewrite R2 in H1. simpl in H1.
-       assert (disjoint {{v}} {{v0}}) by auto.
-       disjoint_solve.
-     split*.
-     intros; apply H2.
-     apply* binds_add_binding.
+     destruct* (IHh _ _ _ _ _ H).
     apply* (@unify_keep_nv h pairs K K' (typ_arrow t1 t2)).
     intros. apply* IHh.
    apply* (@unify_keep_nv h pairs K K' (typ_arrow t1 t2)).
    intros. apply* IHh.
-  destruct* (IHh _ _ _ _ _ H); clear IHh.
+  apply* IHh.
 Qed.
 
 Lemma typ_subst_idem : forall S T,
@@ -415,39 +422,25 @@ Proof.
 Qed.
 
 Lemma unify_types_nv : forall S T1 T2 v T h' pairs' h pairs K K' S',
+  unify_nv (unify h pairs) K S v T = Some (K', S') ->
   typ_subst S T1 = typ_fvar v ->
   typ_subst S T2 = T ->
   unify h' pairs' K S = Some (K', S') ->
-  unify_nv (unify h pairs) K S v T = Some (K', S') ->
   is_subst S ->
   typ_subst S' T1 = typ_subst S' T2.
 Proof.
   intros.
-  unfold unify_nv in H2.
+  unfold unify_nv in H.
   case_rewrite (S.mem v (typ_fv T)) R.
-  assert (is_subst (compose (v ~ T) S)).
-    apply* add_binding_is_subst.
-    use (typ_subst_disjoint T2 H3).
-    rewrite H0 in H4.
-    use (notin_disjoint (mem_3 R)).
-    disjoint_solve.
-  rewrite <- (typ_subst_extend _ _ _ T1 H3 H1).
-  rewrite H.
+  rewrite <- (typ_subst_extend _ _ _ T1 H3 H2).
+  rewrite H0.
   fold kind in *.
   case_rewrite (get_kind v K) R1.
-  rewrite <- (typ_subst_extend _ _ _ (typ_fvar v) H4 H2).
-  rewrite <- (typ_subst_extend _ _ _ T2 H3 H1).
+  assert (is_subst (compose (v ~ T) S)) by auto*.
+  rewrite <- (typ_subst_extend _ _ _ (typ_fvar v) H4 H).
+  rewrite <- (typ_subst_extend _ _ _ T2 H3 H2).
   apply (f_equal (typ_subst S')).
   simpl. destruct* (v==v).
-Qed.
-
-Lemma typ_subst_res_fresh : forall S T v,
-  is_subst S -> typ_subst S T = typ_fvar v -> v # S.
-Proof.
-  intros.
-  use (typ_subst_disjoint T H).
-  rewrite H0 in H1.
-  simpl in H1. destruct* (H1 v).
 Qed.
 
 Theorem unify_types : forall h pairs K S K' S',
@@ -463,40 +456,30 @@ Proof.
     elim H1.
   simpl in H1; destruct H1.
     subst.
+    assert (Hsame: unify h pairs K S = Some (K',S') -> 
+      typ_subst S T1 = typ_subst S T2 -> typ_subst S' T1 = typ_subst S' T2).
+      intros.
+      rewrite <- (typ_subst_extend _ _ _ T1 H0 H').
+      rewrite <- (typ_subst_extend _ _ _ T2 H0 H').
+      congruence.
     case_rewrite (typ_subst S T1) R1; case_rewrite (typ_subst S T2) R2;
       try case_rewrite (S.mem v (typ_fv (typ_bvar n))) R3;
-      try case_rewrite (S.mem v (typ_fv (typ_arrow t t0))) R3.
-          destruct (n === n0).
-            subst.
-            rewrite <- (typ_subst_extend _ _ _ T1 H0 H').
-            rewrite <- (typ_subst_extend _ _ _ T2 H0 H').
-            congruence.
-          discriminate.
-         symmetry.
-         apply* (unify_types_nv _ _ _ _ _ _ _ R2 R1 H' H).
-        apply* (unify_types_nv _ _ _ _ _ _ _ R1 R2 H' H).
-       destruct (v == v0).
-         subst.
-         rewrite <- (typ_subst_extend _ _ _ T1 H0 H').
-         rewrite <- (typ_subst_extend _ _ _ T2 H0 H').
-         congruence.
-       unfold unify_vars in H.
-       destruct (unify_kinds (get_kind v K) (get_kind v0 K)) as [[k1 l]|];
-         try discriminate.
-       assert (IS: is_subst (compose (v ~ typ_fvar v0) S)).
-         apply* add_binding_is_subst.
-         use (typ_subst_disjoint T2 H0).
-         rewrite R2 in H1.
-         disjoint_solve. simpl. destruct* (v1 == v). subst*.
-       rewrite <- (typ_subst_extend _ _ _ T1 IS H).
-       rewrite <- (typ_subst_extend _ _ _ T2 IS H).
-       use (typ_subst_disjoint T1 H0). rewrite  R1 in H1; simpl in H1.
-       repeat rewrite* typ_subst_compose; try (simpl; disjoint_solve).
-       rewrite R1; rewrite R2. simpl.
-       destruct* (v == v). destruct* (v0 == v).
-      apply* (unify_types_nv _ _ _ _ _ _ _ R1 R2 H' H).
-     symmetry.
-     apply* (unify_types_nv _ _ _ _ _ _ _ R2 R1 H' H).
+      try case_rewrite (S.mem v (typ_fv (typ_arrow t t0))) R3;
+      try solve [apply* unify_types_nv];
+      try solve [symmetry; apply* unify_types_nv].
+        destruct* (n === n0).
+        discriminate.
+      destruct (v == v0). subst*.
+      unfold unify_vars in H.
+      destruct (unify_kinds (get_kind v K) (get_kind v0 K)) as [[k1 l]|];
+        try discriminate.
+      assert (IS: is_subst (compose (v ~ typ_fvar v0) S)) by auto*.
+      rewrite <- (typ_subst_extend _ _ _ T1 IS H).
+      rewrite <- (typ_subst_extend _ _ _ T2 IS H).
+      use (typ_subst_disjoint T1 H0). rewrite  R1 in H1; simpl in H1.
+      repeat rewrite* typ_subst_compose; try (simpl; disjoint_solve).
+      rewrite R1; rewrite R2. simpl.
+      destruct* (v == v). destruct* (v0 == v).
     rewrite <- (typ_subst_extend _ _ _ T1 H0 H').
     rewrite <- (typ_subst_extend _ _ _ T2 H0 H').
     rewrite R1; rewrite R2.
@@ -510,68 +493,16 @@ Proof.
     try case_rewrite (S.mem v (typ_fv (typ_arrow t1 t2))) R3;
     fold kind in *;
     try (case_rewrite (get_kind v K) R4);
-    try apply* (IHh _ _ _ _ _ H);
-    try apply* add_binding_is_subst.
-       destruct (n === n0). subst. apply* (IHh _ _ _ _ _ H).
-       discriminate.
-      simpl; intro; auto.
-     simpl; intro; auto.
-    destruct (v == v0).
-      subst.
-      apply* (IHh _ _ _ _ _ H).
-    unfold unify_vars in H.
-    destruct (unify_kinds (get_kind v K) (get_kind v0 K)) as [[k1 l]|];
-      try discriminate.
-    apply* (IHh _ _ _ _ _ H).
-      apply* add_binding_is_subst.
-      use (typ_subst_disjoint t0 H0).
-      rewrite R2 in H2.
-      disjoint_solve.
-      simpl; destruct* (v1 == v). subst*.
-    apply* in_or_app.
-   use (typ_subst_disjoint t0 H0).
-   rewrite R2 in H2.
-   use (notin_disjoint (mem_3 R3)).
-   disjoint_solve.
-  use (typ_subst_disjoint t H0).
-  rewrite R1 in H2.
-  use (notin_disjoint (mem_3 R3)).
-  disjoint_solve.
+    try apply* (IHh _ _ _ _ _ H).
+    destruct* (n === n0).
+    discriminate.
+  destruct* (v == v0).
+  unfold unify_vars in H.
+  destruct (unify_kinds (get_kind v K) (get_kind v0 K)) as [[k1 l]|];
+    try discriminate.
+  apply* IHh.
+  apply* in_or_app.
 Qed.
-
-Section Accum.
-  Variables A B : Set.
-  Variables (f : A -> B) (op : B->B->B) (unit : B).
-
-  Fixpoint accum (l:list A) {struct l} : B :=
-    match l with
-    | nil => unit
-    | a::rem => op (f a) (accum rem)
-    end.
-
-  Variable op_assoc : forall a b c, op a (op b c) = op (op a b) c.
-  Variable op_unit : forall a, op unit a = a.
-
-  Lemma accum_app : forall l2 l1,
-    accum (l1 ++ l2) = op (accum l1) (accum l2).
-  Proof.
-    induction l1; simpl. rewrite* op_unit.
-    rewrite <- op_assoc.
-    rewrite* IHl1.
-  Qed.
-
-End Accum.
-
-Fixpoint all_types S (pairs:list(typ*typ)) {struct pairs} : list typ :=
-  match pairs with
-  | nil => nil
-  | p::rem =>
-      typ_subst S (fst p) :: typ_subst S (snd p) :: all_types S rem
-  end.
-
-Definition all_fv S pairs :=
-  accum typ_fv S.union {} (all_types S pairs).
-Check all_fv.
 
 Lemma kind_subst_idem : forall S k,
   is_subst S -> kind_subst S (kind_subst S k) = kind_subst S k.
@@ -604,8 +535,7 @@ Proof.
 Qed.
 
 Lemma dom_remove_env : forall (A:Set) v (K:Env.env A),
-  ok K ->
- dom (remove_env K v) = S.remove v (dom K).
+  ok K -> dom (remove_env K v) = S.remove v (dom K).
 Proof.
   induction K; simpl; intros.
     apply eq_ext; intros; split; intro. elim (in_empty H0).
@@ -648,115 +578,6 @@ Qed.
 
 Hint Resolve ok_remove_env.
 
-Lemma typ_fv_decr : forall v T S T1,
-  v # S -> disjoint (typ_fv T) ({{v}} \u dom S) ->
-  typ_fv (typ_subst (compose (v ~ T) S) T1) <<
-  S.remove v (typ_fv T \u typ_fv (typ_subst S T1)).
-Proof.
-  intros.
-  rewrite* typ_subst_compose.
-  induction (typ_subst S T1); simpl in *; intros x Hx.
-      elim (in_empty Hx).
-    destruct (v0 == v).
-      subst.
-      apply* S.remove_2.
-        intro Hv; rewrite <- Hv in Hx. destruct* (H0 v).
-        elim H1; auto with sets.
-      auto with sets.
-    apply* S.remove_2.
-      intro Hv; rewrite <- Hv in Hx.
-      revert Hx; simpl*.
-    simpl in Hx; auto with sets.
-  destruct (S.union_1 Hx); [use (IHt1 _ H1) | use (IHt2 _ H1)];
-    apply* remove_subset;
-    intros y Hy; destruct (S.union_1 Hy); auto with sets.
-  simpl. intro x; destruct* (x == v).
-Qed.
-
-Lemma kind_fv_decr : forall v T S k,
-  v # S -> disjoint (typ_fv T) ({{v}} \u dom S) ->
-  kind_fv (kind_subst (compose (v ~ T) S) k) <<
-  S.remove v (typ_fv T \u kind_fv (kind_subst S k)).
-Proof.
-  intros.
-  unfold kind_fv.
-  destruct k as [[kc kv kr kh]|]; simpl.
-    clear kc kv kh.
-    induction kr; simpl; intros x Hx. elim (in_empty Hx).
-    destruct (S.union_1 Hx); clear Hx.
-      rewrite union_assoc.
-      rewrite remove_union.
-      use (typ_fv_decr _ _ _ H H0 H1). auto with sets.
-    rewrite union_assoc.
-    rewrite (union_comm (typ_fv T)).
-    rewrite <- union_assoc.
-    rewrite remove_union.
-    apply S.union_3. apply* IHkr.
-  intros x Hx; elim (in_empty Hx).
-Qed.
-
-Lemma fv_in_decr : forall (A:Set) v T S (E:Env.env A) fv (sub:subs -> A -> A),
-  v # S -> disjoint (typ_fv T) ({{v}} \u dom S) ->
-  (forall a,
-    fv (sub (compose (v ~ T) S) a) << S.remove v (typ_fv T \u fv (sub S a))) ->
-  fv_in fv (map (sub (compose (v ~ T) S)) E) <<
-  S.remove v (typ_fv T \u fv_in fv (map (sub S) E)).
-Proof.
-  intros.
-  induction E; intros x Hx; simpl in *. elim (in_empty Hx).
-  destruct a.
-  simpl in *.
-  destruct (S.union_1 Hx); clear Hx.
-    rewrite union_assoc.
-    rewrite remove_union.
-    apply S.union_2.
-    apply* (H1 a).
-  rewrite union_comm.
-  rewrite <- union_assoc.
-  rewrite remove_union.
-  apply S.union_3.
-  rewrite union_comm.
-  apply* IHE.
-Qed.
-
-Lemma all_fv_decr : forall v T S pairs,
-  v # S -> disjoint (typ_fv T) ({{v}} \u dom S) ->
-  all_fv (compose (v ~ T) S) pairs <<
-  S.remove v (all_fv S ((typ_fvar v, T) :: pairs)).
-Proof.
-  unfold all_fv.
-  induction pairs; intros.
-    simpl. intros x Hx. elim (in_empty Hx).
-  simpl.
-  intros x Hx.
-  rewrite* get_notin_dom.
-  destruct (S.union_1 Hx).
-    use (typ_fv_decr _ _ _ H H0 H1).
-    apply* remove_subset.
-    intros y Hy.
-    destruct (S.union_1 Hy).
-      rewrite <- (@typ_subst_fresh S T) in H3; auto with sets.
-      disjoint_solve.
-    auto with sets.
-  destruct (S.union_1 H1); clear Hx H1.
-    use (typ_fv_decr _ _ _ H H0 H2).
-    apply* remove_subset.
-    intros y Hy.
-    destruct (S.union_1 Hy).
-      rewrite <- (@typ_subst_fresh S T) in H3; auto with sets.
-      disjoint_solve.
-    auto with sets.
-  use (IHpairs H H0 _ H2).
-  apply* remove_subset.
-  simpl.
-  rewrite* get_notin_dom.
-  intros y Hy.
-  clear H1 H2.
-  simpl in Hy.
-  destruct (S.union_1 Hy). auto with sets.
-  destruct (S.union_1 H1); auto with sets.
-Qed.
-
 Definition id := Env.empty (A:=typ).
 
 Lemma typ_subst_id : forall T, typ_subst id T = T.
@@ -769,81 +590,6 @@ Qed.
 Lemma is_subst_id : is_subst id.
 Proof.
   unfold id, is_subst. intro; intros. elim (binds_empty H).
-Qed.
-
-Definition really_all_fv S K pairs :=
-  fv_in kind_fv (map (kind_subst S) K) \u all_fv S pairs.
-
-Lemma really_all_fv_decr : forall S K t t0 pairs v T,
-  really_all_fv S K ((t, t0) :: pairs) \u fv_in typ_fv S << dom K ->
-  typ_subst S t = typ_fvar v ->
-  typ_subst S t0 = T ->
-  is_subst S ->
-  ok K ->
-  S.mem v (typ_fv T) = false ->
-  really_all_fv (compose (v ~ T) S) (remove_env K v) pairs \u
-  fv_in typ_fv (compose (v ~ T) S) << S.remove v (dom K).
-Proof.
-  intros until T. intros Hra R1 R2 HS HK R3.
-  unfold really_all_fv in *.
-  intros x Hx.
-  apply* remove_subset.
-  clear Hra.
-  assert (v # S) by apply* typ_subst_res_fresh.
-  assert (disjoint (typ_fv T) ({{v}} \u dom S)).
-    use (typ_subst_disjoint t0 HS). rewrite R2 in H0.
-    disjoint_solve.
-    destruct* (v0 == v); subst*.
-  destruct (S.union_1 Hx); clear Hx.
-    rewrite remove_union; apply S.union_2.
-    destruct (S.union_1 H1); clear H1.
-      unfold all_fv; simpl. rewrite R2.
-      rewrite (union_comm (typ_fv (typ_subst S t))).
-      do 2 rewrite union_assoc. do 2 (rewrite remove_union; apply S.union_2).
-      rewrite union_comm.
-      refine (fv_in_decr _ _ _ _ _ _ _ _ _); auto.
-      intros; apply* kind_fv_decr.
-      clear -H2; induction K; simpl in *. auto.
-      destruct a; simpl.
-      destruct (v == v0); simpl in H2.
-        auto with sets.
-      destruct (S.union_1 H2); auto with sets.
-    rewrite remove_union; apply S.union_3.
-    unfold all_fv; simpl.
-    rewrite <- (typ_subst_idem t HS).
-    rewrite <- (typ_subst_idem t0 HS).
-    rewrite R1; rewrite R2.
-    apply (all_fv_decr _ _ _ H H0 H2).
-  unfold all_fv; simpl. rewrite R2.
-  rewrite (union_comm (typ_fv T)).
-  do 3 rewrite <- union_assoc.
-  do 3 (rewrite remove_union; apply S.union_3).
-  unfold compose in H1.
-  simpl in H1.
-  destruct (S.union_1 H1).
-    rewrite remove_union.
-    rewrite remove_notin. auto with sets.
-    destruct* (H0 v).
-  replace S with (map (typ_subst id) S).
-    replace (v~T) with (compose (v~T) id) in H2.
-      assert (v # id) by (unfold id; auto).
-      assert (disjoint (typ_fv T) ({{v}} \u dom id))
-        by (simpl; disjoint_solve).
-      refine (fv_in_decr _ _ _ _ _ _ _ _ _); auto.
-      intros; apply* typ_fv_decr.
-    reflexivity.
-  clear; induction S; simpl; auto.
-  destruct a; simpl; rewrite typ_subst_id; rewrite* IHS.
-Qed.
-
-Lemma really_all_fv_comm : forall S K t t0 pairs,
-  really_all_fv S K ((t,t0)::pairs) = really_all_fv S K ((t0,t)::pairs).
-Proof.
-  intros.
-  unfold really_all_fv, all_fv; simpl.
-  rewrite (union_assoc (typ_fv (typ_subst S t))).
-  rewrite (union_comm (typ_fv (typ_subst S t))).
-  rewrite* <- (union_assoc (typ_fv (typ_subst S t0))).
 Qed.
 
 Lemma binds_remove_env : forall (A:Set) v K x (a:A),
@@ -902,10 +648,24 @@ Definition well_subst K K' S :=
 Definition unify_kinds_spec K S K' S' :=
   is_subst S -> ok K ->
   disjoint (dom S) (dom K) ->
-  (* really_all_fv S K pairs \u fv_in typ_fv S << dom K -> *)
   ok K' /\ disjoint (dom S') (dom K') /\
-  (* fv_in kind_fv (map (kind_subst S') K') \u fv_in typ_fv S' << dom K' /\ *)
   well_subst (map (kind_subst S) K) (map (kind_subst S') K') S'.
+
+Lemma disjoint_add_binding : forall v T S (K:kenv),
+  is_subst S -> ok K ->
+  disjoint (dom S) (dom K) ->
+  disjoint (dom (compose (v ~ T) S)) (dom (remove_env K v)).
+Proof.
+  intros.
+  rewrite* dom_remove_env.
+  unfold compose. simpl.
+  rewrite dom_map.
+  intro x; destruct (v == x).
+    right; apply* S.remove_1.
+  destruct* (H1 x). right; intro. elim H2; apply* S.remove_3.
+Qed.
+
+Hint Resolve disjoint_add_binding.
 
 Lemma unify_kinds_nv : forall h pairs K S v T K' S' h' pairs' t t0,
   unify_nv (unify h pairs) K S v T = Some (K', S') ->
@@ -914,28 +674,16 @@ Lemma unify_kinds_nv : forall h pairs K S v T K' S' h' pairs' t t0,
   unify h' pairs' K S = Some (K',S') ->
   (forall pairs K S,
     unify h pairs K S = Some (K',S') -> unify_kinds_spec K S K' S') ->
-  unify_kinds_spec (* (t,t0)::pairs *) K S K' S'.
+  unify_kinds_spec K S K' S'.
 Proof.
   unfold unify_nv.
   intros until 1.
   intros R1 R2 H' IHh HS Hok Dis (* Hra *).
   case_rewrite (S.mem v (typ_fv T)) R3.
   case_rewrite (get_kind v K) R4.
-  assert (His : is_subst (compose (v ~ T) S)).
-    apply* add_binding_is_subst.
-    use (typ_subst_disjoint t0 HS).
-    rewrite R2 in H0.
-    use (notin_disjoint (mem_3 R3)).
-    disjoint_solve.
   destruct* (IHh _ _ _ H); clear IHh.
-    rewrite* dom_remove_env.
-    unfold compose. simpl.
-    rewrite dom_map.
-    intro x; destruct (v == x).
-      right; apply* S.remove_1.
-    destruct* (Dis x). right; intro. elim H0; apply* S.remove_3.
-    (* rewrite* dom_remove_env. apply* really_all_fv_decr. *)
   intuition.
+  assert (His : is_subst (compose (v ~ T) S)) by auto*.
   clear H0 H2 R1 R2 R3 Dis.
   intro; intros.
   unfold well_subst in H3.
@@ -953,28 +701,6 @@ Proof.
   intro; apply* typ_subst_extend.
 Qed.
 
-Lemma in_all_fv : forall S t t0 l,
-  In (t,t0) l ->
-  typ_fv (typ_subst S t) \u typ_fv (typ_subst S t0) << all_fv S l.
-Proof.
-  induction l; simpl; intros H x Hx. elim H.
-  unfold all_fv; simpl.
-  destruct H.
-    subst; simpl.
-    rewrite union_assoc; auto with sets.
-  rewrite union_assoc; apply S.union_3; apply* IHl.
-Qed.
-
-Lemma in_typ_fv : forall t l,
-  In t l -> typ_fv t << typ_fv_list l.
-Proof.
-  induction l; simpl; intros H x Hx. elim H.
-  destruct H.
-    subst; simpl.
-    auto with sets.
-  apply S.union_3; apply* IHl.
-Qed.
-
 Lemma get_in : forall (A:Set) x (a:A) E,
   binds x a E -> In (x, a) E.
 Proof.
@@ -983,63 +709,13 @@ Proof.
   destruct* (x == v). inversions* H.
 Qed.
 
-Lemma unify_kinds_fv : forall k k0 k1 l S,
-  unify_kinds k k0 = Some (k1, l) ->
-  kind_fv (kind_subst S k1) \u all_fv S l <<
-  kind_fv (kind_subst S k) \u kind_fv (kind_subst S k0).
-Proof.
-  unfold unify_kinds; intros.
-  destruct k as [[kc kv kr kh]|].
-    destruct k0 as [[kc0 kv0 kr0 kh0]|].
-      destruct (cstr_valid (cstr_lub kc kc0)); try discriminate.
-      inversions H; clear H.
-      simpl.
-      unfold kind_fv; simpl.
-      repeat rewrite map_map; simpl.
-      rewrite <- fv_list_map. rewrite <- map_app.
-      set (pairs := nil(A:=typ*typ)).
-      set (kr' := nil(A:=var*typ)).
-      intros x Hx.
-      rewrite <- union_empty_r.
-      replace {} with
-        (typ_fv_list (List.map (fun x : var * typ => typ_subst S (snd x)) kr'))
-        by reflexivity.
-      rewrite <- union_empty_r.
-      replace {} with (all_fv S pairs) by reflexivity.
-      clearbody pairs kr'.
-      gen pairs kr'; induction (kr ++ kr0); simpl; intros.
-        rewrite <- union_assoc; auto with sets.
-      destruct a; simpl in *.
-      destruct (In_dec eq_var_dec v0 (unique (cstr_lub kc kc0))).
-        case_rewrite (get v0 kr') R1;
-          poses Hsub (IHl _ _ Hx); clear IHl.
-          rewrite <- union_assoc in Hsub.
-          destruct (S.union_1 Hsub); clear Hsub; auto with sets.
-          destruct (S.union_1 H); clear H; auto with sets.
-          unfold all_fv in H0; simpl in H0.
-          destruct (S.union_1 H0); clear H0; auto with sets.
-          destruct (S.union_1 H); clear H; auto with sets.
-          use (get_in R1).
-          use (in_map (fun x : var * typ => typ_subst S (snd x)) _ _ H).
-          use (in_typ_fv _ _ H1 H0).
-          auto with sets.
-        simpl in Hsub. union_solve x.
-      poses Hsub (IHl _ _ Hx); clear IHl Hx.
-      simpl in Hsub.
-      union_solve x.
-    inversions H.
-    unfold kind_fv, all_fv; simpl.
-    apply subset_refl.
-  inversions H.
-  unfold kind_fv, all_fv; simpl.
-  rewrite union_comm; apply subset_refl.
-Qed.
-
 Definition kind_entails k k' :=
-  match k', k with
-  | None, _ => True
-  | Some c', Some c => entails c c'
-  | Some c', None => False
+  match k' with
+  | None => True
+  | Some c' => match k with
+               | Some c => entails c c'
+               | None => False
+               end
   end.
 
 Lemma unify_kind_rel_keep : forall kr kr' un pairs k' l,
@@ -1101,16 +777,6 @@ Proof.
    inversions H; clear H.
    simpl. apply entails_refl.
   auto.
-Qed.
-
-Lemma all_fv_app : forall S l1 l2,
-  all_fv S (l1 ++ l2) = all_fv S l1 \u all_fv S l2.
-Proof.
-  intros.
-  unfold all_fv.
-  induction l1; simpl. rewrite* union_empty_l.
-  rewrite IHl1.
-  repeat rewrite union_assoc. auto.
 Qed.
 
 Lemma map_remove_env : forall (A:Set) x f (E:Env.env A),
@@ -1339,39 +1005,11 @@ Lemma unify_kinds_vars :
 Proof.
   intros until l.
   intros H R1 R2 n R3 H' IHh HS HK Dis (* Hra *).
-  assert (His: is_subst (compose (v ~ typ_fvar v0) S)).
-    apply* add_binding_is_subst.
-    use (typ_subst_disjoint t0 HS).
-    rewrite R2 in H0.
-    simpl in *.
-    intro x. destruct* (x == v0). subst v0; destruct* (H0 x).
+  assert (His: is_subst (compose (v ~ typ_fvar v0) S)) by auto*.
   destruct* (IHh _ _ _ H); clear IHh.
       constructor. repeat apply ok_remove_env. auto.
-      rewrite dom_remove_env.
-        apply S.remove_1. reflexivity.
-      apply* ok_remove_env.
-        (* intros. binds_cases H0.
-          use (ok_remove_env v HSK).
-          use (binds_orig_remove_env _ H0 B).
-          use (binds_orig_remove_env _ HSK H1).
-          subst.
-          destruct (binds_map_inv _ _ H2) as [k' [HE HB]].
-          destruct k' as [[kc kr]|]; try discriminate.
-          use (proj2 HK _ _ HB).
-          simpl in HE; inversions HE.
-          apply* kind_ok_map.
-        destruct (binds_single_inv B0); subst k1. clear B0 H0 H2.
-        apply (kind_ok_unify_kinds _ _ R5).
-          subst.
-          destruct (binds_map_inv _ _ R3) as [k' [HE HB]]. subst.
-          destruct k' as [[kc kr]|]; simpl*.
-          apply kind_ok_map.
-          apply (proj2 HK _ _ HB).
-        subst.
-        destruct (binds_map_inv _ _ R4) as [k' [HE HB]]. subst.
-        destruct k' as [[kc kr]|]; simpl*.
-        apply kind_ok_map.
-        apply (proj2 HK _ _ HB). *)
+      rewrite* dom_remove_env.
+      apply S.remove_1. reflexivity.
     simpl.
     repeat rewrite* dom_remove_env.
     rewrite dom_map.
@@ -1382,90 +1020,14 @@ Proof.
       elim (S.remove_1 (refl_equal v) H0).
     destruct* (x == v0).
       subst; left.
-      use (typ_subst_res_fresh _ HS R2).
+      assert (v0 # S). use (typ_subst_res_fresh _ HS R2). auto.
     destruct* (Dis x).
     right; apply* notin_union_l.
     intro.
     use (S.remove_3 (S.remove_3 H1)).
-    (* assert (S.mem v (typ_fv (typ_fvar v0)) = false).
-      simpl. case_eq (S.mem v {{v0}}); intros; auto.
-      pose (S.mem_2 H0).
-      elim n; rewrite* (S.singleton_1 i).
-    poses Hsub (really_all_fv_decr Hra R1 R2 HS Hok H0).
-    intros x Hx.
-    unfold really_all_fv in Hx.
-    rewrite all_fv_app in Hx.
-    simpl in Hx.
-    repeat rewrite union_assoc in Hx.
-    simpl.
-    rewrite* dom_remove_env.
-    destruct (x == v0). subst; auto with sets.
-    rewrite* dom_remove_env.
-    rewrite HeqSK; rewrite dom_map.
-    assert (v # S) by apply* typ_subst_res_fresh.
-    assert (disjoint (typ_fv (typ_fvar v0)) ({{v}} \u dom S)).
-      simpl; intro y; destruct* (y == v0); subst.
-      use (typ_subst_res_fresh _ HS R2).
-    assert (forall y k,
-              binds y k SK ->
-              x \in kind_fv (kind_subst (compose (v ~ typ_fvar v0) S) k) ->
-              x \in {{v0}} \u S.remove v0 (S.remove v (dom K))).
-      clear Hx; intros.
-      use (kind_fv_decr _ _ _ H1 H2 H4).
-      simpl in H5; rewrite remove_union in H5.
-      destruct (S.union_1 H5); clear H4 H5.
-        apply S.union_2; apply* S.remove_3.
-      apply S.union_3; apply* S.remove_2.
-      apply S.remove_2. intro Hv; elim (S.remove_1 Hv H6).
-      apply Hra.
-      unfold really_all_fv.
-      repeat apply S.union_2.
-      use (S.remove_3 H6).
-      rewrite <- HeqSK.
-      apply (fv_in_spec kind_fv H3).
-      rewrite HeqSK in H3.
-      destruct (binds_map_inv _ _ H3) as [k' [E B]].
-      subst.
-      rewrite kind_subst_idem in H4; auto.
-    union_solve x.
-            poses Hfv (unify_kinds_fv _ _ _ R5 (S.union_2 _ H4)); clear H4.
-            destruct (S.union_1 Hfv); clear Hfv. apply* (H3 _ _ R3 H4).
-            apply* H3.
-          apply S.union_3.
-          apply S.remove_2. intro Hx; elim n0; rewrite* Hx.
-          apply Hsub.
-          apply S.union_2.
-          clear H H' Hsub Hra; unfold really_all_fv in *.
-          apply S.union_2.
-          subst.
-          repeat rewrite map_remove_env in *.
-          rewrite <- (map_map_env (kind_subst (compose (v ~ typ_fvar v0) S)))
-            in H4.
-            apply (fv_in_remove_env _ _ _ H4).
-          intro.
-          rewrite (kind_subst_combine (compose (v ~ typ_fvar v0) S)). auto.
-          intro.
-          assert (disjoint (dom (v ~ typ_fvar v0)) (dom S)).
-            simpl. use (typ_subst_res_fresh _ HS R1).
-            intro y; destruct* (y == v).
-          repeat rewrite* typ_subst_compose. rewrite* typ_subst_idem.
-        poses Hfv (unify_kinds_fv _ _ _ R5 (S.union_3 _ H5)).
-        destruct (S.union_1 Hfv); clear Hfv. apply* (H3 _ _ R3 H4).
-        apply* H3.
-      unfold really_all_fv in Hsub.
-      apply S.union_3.
-      apply S.remove_2. intro Hx; elim n0; rewrite* Hx.
-      apply Hsub; clear H H' Hra Hsub.
-      auto with sets.
-    unfold really_all_fv in Hsub.
-    apply S.union_3.
-    apply S.remove_2. intro Hx; elim n0; rewrite* Hx.
-    apply Hsub; clear H H' Hra Hsub.
-    unfold compose. simpl.
-    auto with sets. *)
   intuition.
   subst; apply* well_subst_unify.
-  apply* typ_subst_res_fresh.
+  use (typ_subst_res_fresh _ HS R1).
 Qed.
 
 Theorem unify_kinds_ok : forall h pairs K S K' S',
@@ -1478,9 +1040,6 @@ Proof.
   destruct pairs.
     inversions H; clear H.
     intuition.
-      (* intros x Hx; apply Hra.
-      unfold really_all_fv.
-      destruct (S.union_1 Hx); auto with sets. *)
     intro; intros.
     destruct (binds_map_inv _ _ H) as [k' [Ek' Bk']]; subst k.
     rewrite* kind_subst_idem.
@@ -1494,21 +1053,12 @@ Proof.
   case_rewrite (typ_subst S t) R1; case_rewrite (typ_subst S t0) R2.
         destruct (n === n0).
           apply* (IHh _ _ _ _ _ H).
-          (* intros x Hx; apply Hra.
-          clear -Hx.
-          unfold really_all_fv, all_fv in *; simpl.
-          union_solve x. *)
         discriminate.
-       (* rewrite really_all_fv_comm in Hra. *)
        refine (unify_kinds_nv h _ _ _ _ _ H R2 R1 H' _ _ _ _); auto*.
       refine (unify_kinds_nv h _ _ _ _ _ H R1 R2 H' _ _ _ _); auto*.
       destruct (v == v0).
         subst.
         apply* (IHh _ _ _ _ _ H).
-        (* intros x Hx; apply Hra.
-        clear -Hx.
-        unfold really_all_fv, all_fv in *; simpl.
-        union_solve x. *)
       unfold unify_vars in H.
       case_rewrite (unify_kinds (get_kind v K) (get_kind v0 K)) R3.
       destruct p.
@@ -1518,15 +1068,6 @@ Proof.
      refine (unify_kinds_nv h _ _ _ _ _ H R1 R2 H' _ _ _ _); auto*.
     refine (unify_kinds_nv h _ _ _ _ _ H R2 R1 H' _ _ _ _); auto*.
   destruct* (IHh _ _ _ _ _ H HS).
-  (* clear -Hra R1 R2 HS.
-  unfold really_all_fv, all_fv in *; simpl in *.
-  intros x Hx; apply Hra; clear Hra.
-  rewrite <- (typ_subst_idem t HS).
-  rewrite <- (typ_subst_idem t0 HS).
-  rewrite R1; rewrite R2.
-  simpl.
-  repeat rewrite <- union_assoc in *.
-  union_solve x. *)
 Qed.
        
 Lemma typ_subst_map_idem : forall S,
@@ -1626,6 +1167,13 @@ Proof.
   intro; symmetry; apply* typ_subst_compose.
 Qed.
 
+Lemma typ_subst_res_fresh' : forall S T v,
+  is_subst S -> typ_subst S T = typ_fvar v -> v # S.
+Proof.
+  intros.
+  use (typ_subst_res_fresh _ H H0).
+Qed.
+
 Lemma unify_mgu_nv : forall K0 S0 pairs K S h t t0 v T,
   typ_subst S0 t = typ_fvar v ->
   typ_subst S0 t0 = T ->
@@ -1641,7 +1189,7 @@ Proof.
     use (Heq _ _ H); clear H.
     rewrite R1 in H0; rewrite R2 in H0.
     auto.
-  assert (Hv: v # S0) by apply* typ_subst_res_fresh.
+  assert (Hv: v # S0) by apply* typ_subst_res_fresh'.
   unfold unify_nv in HU.
   case_rewrite (S.mem v (typ_fv T)) R3.
   case_rewrite (get_kind v K0) R4.
@@ -1653,13 +1201,6 @@ Proof.
       reflexivity.
     congruence.
   destruct* (IHh _ _ HU).
-        apply* add_binding_is_subst.
-        assert (disjoint {{v}} (typ_fv T)).
-          intro x; destruct* (x == v); subst.
-          right; intro. rewrite (S.mem_1 H) in R3. discriminate.
-        use (typ_subst_disjoint t0 HS0).
-        rewrite R2 in H0.
-        disjoint_solve.
       intros.
       repeat rewrite* typ_subst_compose.
       assert (In (T1, T2) ((t,t0)::pairs)) by simpl*.
@@ -1822,8 +1363,8 @@ Proof.
     use (Heq _ _ H); clear H.
     rewrite R1 in H0; rewrite R2 in H0.
     auto.
-  assert (Hv: v # S0) by apply* typ_subst_res_fresh.
-  assert (Hv0: v0 # S0) by apply* typ_subst_res_fresh.
+  assert (Hv: v # S0) by apply* typ_subst_res_fresh'.
+  assert (Hv0: v0 # S0) by apply* typ_subst_res_fresh'.
   unfold unify_vars in R3.
   case_rewrite (unify_kinds (get_kind v K0) (get_kind v0 K0)) R4.
   destruct p.
@@ -1841,15 +1382,6 @@ Proof.
     assert (ok (remove_env K0 v)) by auto.
     apply (@ok_push _ _ v0 k (ok_remove_env v0 H)).
     rewrite* dom_remove_env. apply S.remove_1. reflexivity.
-(*  assert (Bsi: forall v,
-            get_kind v (kS0 K0) = kind_subst S0 (get_kind v (kS0 K0))).
-    clear -HS0; intro.
-    unfold get_kind.
-    case_eq (get v (kS0 K0)); intros; simpl*.
-    unfold kS0.
-    destruct (binds_map_inv _ _ H). destruct H0.
-    subst.
-    rewrite* kind_subst_idem. *)
   poses Wk (well_subst_get_kind v WS).
   rewrite <- Sv in Wk.
   simpl typ_subst in Wk. destruct* (v == v). clear e.
@@ -1866,12 +1398,6 @@ Proof.
       rewrite <- H1; simpl in H; rewrite H in H2; inversions H2;
       rewrite* (binds_get_kind H4).
   destruct* (IHh _ _ _ HU).
-        apply* add_binding_is_subst.
-        simpl.
-        assert (disjoint {{v}} {{v0}}). intro x; destruct* (x == v). subst*.
-        use (typ_subst_disjoint t0 HS0).
-        rewrite R2 in H1.
-        simpl in H1; disjoint_solve.
       intros.
       repeat rewrite* typ_subst_compose.
       repeat rewrite Sv.
@@ -2004,6 +1530,39 @@ End Mgu.
 
 Check unify_mgu.
 
+Section Accum.
+  Variables A B : Set.
+  Variables (f : A -> B) (op : B->B->B) (unit : B).
+
+  Fixpoint accum (l:list A) {struct l} : B :=
+    match l with
+    | nil => unit
+    | a::rem => op (f a) (accum rem)
+    end.
+
+  Variable op_assoc : forall a b c, op a (op b c) = op (op a b) c.
+  Variable op_unit : forall a, op unit a = a.
+
+  Lemma accum_app : forall l2 l1,
+    accum (l1 ++ l2) = op (accum l1) (accum l2).
+  Proof.
+    induction l1; simpl. rewrite* op_unit.
+    rewrite <- op_assoc.
+    rewrite* IHl1.
+  Qed.
+
+End Accum.
+
+Fixpoint all_types S (pairs:list(typ*typ)) {struct pairs} : list typ :=
+  match pairs with
+  | nil => nil
+  | p::rem =>
+      typ_subst S (fst p) :: typ_subst S (snd p) :: all_types S rem
+  end.
+
+Definition all_fv S pairs :=
+  accum typ_fv S.union {} (all_types S pairs).
+
 Fixpoint typ_size (T : typ) : nat :=
   match T with
   | typ_arrow T1 T2 => S (typ_size T1 + typ_size T2)
@@ -2053,6 +1612,9 @@ Proof.
   omega.
 Qed.
 
+Definition really_all_fv S K pairs :=
+  fv_in kind_fv (map (kind_subst S) K) \u all_fv S pairs.
+
 Definition size_pairs S K pairs :=
   pow2exp (all_size S K pairs) (S.cardinal (really_all_fv S K pairs)).
 
@@ -2069,9 +1631,118 @@ Proof.
   intros x Hx; union_solve x.
 Qed.
 
-Lemma really_all_fv_decr' : forall S K pairs v T,
+Lemma typ_fv_decr : forall v T S T1,
+  v # S -> disjoint (typ_fv T) ({{v}} \u dom S) ->
+  typ_fv (typ_subst (compose (v ~ T) S) T1) <<
+  S.remove v (typ_fv T \u typ_fv (typ_subst S T1)).
+Proof.
+  intros.
+  rewrite* typ_subst_compose.
+  induction (typ_subst S T1); simpl in *; intros x Hx.
+      elim (in_empty Hx).
+    destruct (v0 == v).
+      subst.
+      apply* S.remove_2.
+        intro Hv; rewrite <- Hv in Hx. destruct* (H0 v).
+        elim H1; auto with sets.
+      auto with sets.
+    apply* S.remove_2.
+      intro Hv; rewrite <- Hv in Hx.
+      revert Hx; simpl*.
+    simpl in Hx; auto with sets.
+  destruct (S.union_1 Hx); [use (IHt1 _ H1) | use (IHt2 _ H1)];
+    apply* remove_subset;
+    intros y Hy; destruct (S.union_1 Hy); auto with sets.
+  simpl. intro x; destruct* (x == v).
+Qed.
+
+Lemma kind_fv_decr : forall v T S k,
+  v # S -> disjoint (typ_fv T) ({{v}} \u dom S) ->
+  kind_fv (kind_subst (compose (v ~ T) S) k) <<
+  S.remove v (typ_fv T \u kind_fv (kind_subst S k)).
+Proof.
+  intros.
+  unfold kind_fv.
+  destruct k as [[kc kv kr kh]|]; simpl.
+    clear kc kv kh.
+    induction kr; simpl; intros x Hx. elim (in_empty Hx).
+    destruct (S.union_1 Hx); clear Hx.
+      rewrite union_assoc.
+      rewrite remove_union.
+      use (typ_fv_decr _ _ _ H H0 H1). auto with sets.
+    rewrite union_assoc.
+    rewrite (union_comm (typ_fv T)).
+    rewrite <- union_assoc.
+    rewrite remove_union.
+    apply S.union_3. apply* IHkr.
+  intros x Hx; elim (in_empty Hx).
+Qed.
+
+Lemma fv_in_decr : forall (A:Set) v T S (E:Env.env A) fv (sub:subs -> A -> A),
+  v # S -> disjoint (typ_fv T) ({{v}} \u dom S) ->
+  (forall a,
+    fv (sub (compose (v ~ T) S) a) << S.remove v (typ_fv T \u fv (sub S a))) ->
+  fv_in fv (map (sub (compose (v ~ T) S)) E) <<
+  S.remove v (typ_fv T \u fv_in fv (map (sub S) E)).
+Proof.
+  intros.
+  induction E; intros x Hx; simpl in *. elim (in_empty Hx).
+  destruct a.
+  simpl in *.
+  destruct (S.union_1 Hx); clear Hx.
+    rewrite union_assoc.
+    rewrite remove_union.
+    apply S.union_2.
+    apply* (H1 a).
+  rewrite union_comm.
+  rewrite <- union_assoc.
+  rewrite remove_union.
+  apply S.union_3.
+  rewrite union_comm.
+  apply* IHE.
+Qed.
+
+Lemma all_fv_decr : forall v T S pairs,
+  v # S -> disjoint (typ_fv T) ({{v}} \u dom S) ->
+  all_fv (compose (v ~ T) S) pairs <<
+  S.remove v (all_fv S ((typ_fvar v, T) :: pairs)).
+Proof.
+  unfold all_fv.
+  induction pairs; intros.
+    simpl. intros x Hx. elim (in_empty Hx).
+  simpl.
+  intros x Hx.
+  rewrite* get_notin_dom.
+  destruct (S.union_1 Hx).
+    use (typ_fv_decr _ _ _ H H0 H1).
+    apply* remove_subset.
+    intros y Hy.
+    destruct (S.union_1 Hy).
+      rewrite <- (@typ_subst_fresh S T) in H3; auto with sets.
+      disjoint_solve.
+    auto with sets.
+  destruct (S.union_1 H1); clear Hx H1.
+    use (typ_fv_decr _ _ _ H H0 H2).
+    apply* remove_subset.
+    intros y Hy.
+    destruct (S.union_1 Hy).
+      rewrite <- (@typ_subst_fresh S T) in H3; auto with sets.
+      disjoint_solve.
+    auto with sets.
+  use (IHpairs H H0 _ H2).
+  apply* remove_subset.
+  simpl.
+  rewrite* get_notin_dom.
+  intros y Hy.
+  clear H1 H2.
+  simpl in Hy.
+  destruct (S.union_1 Hy). auto with sets.
+  destruct (S.union_1 H1); auto with sets.
+Qed.
+
+Lemma really_all_fv_decr : forall S K pairs v T,
   v # S -> disjoint (typ_fv T) ({{v}} \u dom S) -> ok K ->
-  really_all_fv (compose (v ~ T) S) (remove_env K v) pairs <<
+  really_all_fv (compose (v ~ T) S) K pairs <<
   S.remove v (really_all_fv S K ((typ_fvar v, T) :: pairs)).
 Proof.
   intros until T. intros Hv Dis HK.
@@ -2089,8 +1760,6 @@ Proof.
   rewrite* typ_subst_fresh; try disjoint_solve.
   refine (fv_in_decr _ _ _ _ _ _ _ _ _); auto.
     intros; apply* kind_fv_decr.
-  rewrite map_remove_env in H.
-  refine (fv_in_remove_env _ _ _ H).
 Qed.
 
 Lemma cardinal_decr : forall v T S K pairs,
@@ -2099,9 +1768,16 @@ Lemma cardinal_decr : forall v T S K pairs,
   S.cardinal (really_all_fv S K ((typ_fvar v, T) :: pairs)).
 Proof.
   intros.
-  use (really_all_fv_decr' (pairs:=pairs) H H0 H1).
+  use (really_all_fv_decr (pairs:=pairs) H H0 H1).
   use (le_lt_n_Sm _ _ (cardinal_subset H2)).
-  rewrite cardinal_remove in H3. auto.
+  rewrite cardinal_remove in H3.
+    eapply le_lt_trans; try apply H3.
+    apply cardinal_subset.
+    unfold really_all_fv. rewrite map_remove_env.
+    intros x Hx.
+    destruct (S.union_1 Hx).
+      apply S.union_2. refine (fv_in_remove_env _ _ _ H4).
+    auto with sets.
   unfold really_all_fv, all_fv; simpl.
   rewrite* get_notin_dom.
   simpl; auto with sets.
@@ -2245,9 +1921,24 @@ Proof.
   rewrite* typ_subst_idem.
 Qed.
 
+Lemma accum_le : forall (A:Set) f (a:A) l,
+  In a l -> f a <= accum f plus 0 l.
+Proof.
+  induction l; simpl; intros. elim H.
+  destruct H. subst; omega.
+  use (IHl H). omega.
+Qed.
+
+Lemma length_accum : forall (A:Set) l,
+  length l = accum (fun x:A => 1) plus 0 l.
+Proof.
+  induction l; simpl; congruence.
+Qed.
+
 Lemma unify_kinds_size : forall k k0 k1 l S,
   unify_kinds k k0 = Some (k1, l) ->
-  length (kind_types k1) <= length (kind_types k ++ kind_types k0) /\
+  (forall f, accum f plus 0 (kind_types k1)
+    <= accum f plus 0 (kind_types k ++ kind_types k0)) /\
   accum typ_size plus 0 (all_types S l) + kinds_size S (kind_types k1) <=
   kinds_size S (kind_types k ++ kind_types k0).
 Proof.
@@ -2280,7 +1971,7 @@ Proof.
        destruct* (In_dec eq_var_dec v un).
        case_rewrite (get v kr') R1; simpl*.
        destruct (IHl ((t,t0)::pairs) kr'); clear IHl.
-       split. omega.
+       split. intros; use (H1 f); omega.
        eapply le_trans; try apply H2. clear H2.
        unfold kinds_size; simpl.
        fold (typ_size' S t). fold (typ_size' S t0).
@@ -2293,42 +1984,187 @@ Proof.
        repeat rewrite plus_assoc.
        apply plus_le_compat_r.
        rewrite map_app. rewrite accum_app; try (intros; omega).
-Lemma accum_le : forall (A:Set) f (a:A) l,
-  In a l -> f a <= accum f plus 0 l.
-Proof.
-  induction l; simpl; intros. elim H.
-  destruct H. subst; omega.
-  use (IHl H). omega.
-Qed.
        use (in_map (fun x : var * typ => snd x) _ _ (get_in R1)).
        simpl in H2.
        eapply le_trans. apply (accum_le (typ_size' S) _ _ H2).
        rewrite <- plus_assoc.
        refine (le_trans _ _ _ _ (le_plus_r _ _)).
        apply le_plus_l.
-       
-       destruct (IHl pairs ((v,t)::kr')); clear IHl.
-       assert
-         (length (List.map (fun x : var * typ => snd x) (l ++ (v, t) :: kr')) <=
-           (length (t :: List.map (fun x : var * typ => snd x) (l ++ kr')))).
-         simpl.
-         repeat rewrite map_length.
-         repeat rewrite app_length.
-         simpl. omega.
-       split.
-         eapply le_trans. apply H0. apply H2.
-       eapply le_trans. apply H1.
-       apply plus_le_compat_l.
-       clear -H2.
-       unfold kinds_size.
-       eapply le_trans.
-         apply mult_le_compat_r. apply H2.
-       apply mult_le_compat_l.
-       clear; repeat rewrite map_app.
-       simpl; repeat rewrite accum_app; simpl; intros; omega.
+     assert (forall a (b:list(var*typ)*list(typ*typ)),
+       (if In_dec eq_var_dec v un
+        then match get v kr' with Some T' => a T' | None => b end
+        else b) = b).
+       intros.
+       destruct* (In_dec eq_var_dec v un).
+       destruct* H. rewrite* H.
+     rewrite H0; clear H H0.
      destruct (IHl pairs ((v,t)::kr')); clear IHl.
-     
+     assert
+       (length (List.map (fun x : var * typ => snd x) (l ++ (v, t) :: kr')) <=
+         (length (t :: List.map (fun x : var * typ => snd x) (l ++ kr')))).
+       simpl.
+       repeat rewrite map_length.
+       repeat rewrite app_length.
+       simpl. omega.
+     split.
+       intros; eapply le_trans. apply (H f).
+       repeat rewrite map_app; simpl.
+       repeat rewrite accum_app; simpl; intros; omega.
+     eapply le_trans. apply H0.
+     apply plus_le_compat_l.
+     clear -H1.
+     unfold kinds_size.
+     eapply le_trans.
+       apply mult_le_compat_r. apply H1.
+     apply mult_le_compat_l.
+     clear; repeat rewrite map_app.
+     simpl; repeat rewrite accum_app; simpl; intros; omega.
+    inversions H; simpl. rewrite* <- app_nil_end.
+   inversions H; simpl*.
+  inversions H; simpl*.
+Qed.
 
+Lemma accum_remove_env : forall f v K,
+  accum f plus 0 (kind_types (get_kind v K) ++ kenv_types (remove_env K v)) =
+  accum f plus 0 (kenv_types K).
+Proof.
+  induction K; simpl. auto.
+  destruct a; simpl.
+  unfold get_kind in *. simpl.
+  destruct (v == v0). auto.
+  simpl.
+  repeat (rewrite accum_app in *; try (intros; omega)).
+Qed.
+
+Lemma length_remove_env : forall v K,
+  length (kind_types (get_kind v K) ++ kenv_types (remove_env K v)) =
+  length (kenv_types K).
+Proof.
+  intros; repeat rewrite length_accum.
+  apply accum_remove_env.
+Qed.
+
+Lemma all_types_app : forall S l1 l2,
+  all_types S (l1 ++ l2) = all_types S l1 ++ all_types S l2.
+Proof.
+  intros; induction l1; simpl. auto.
+  rewrite* <- IHl1.
+Qed.
+
+Lemma typ_size'_var : forall v v0 T,
+  typ_size (typ_subst (v ~ typ_fvar v0) T) = typ_size T.
+Proof.
+  induction T; simpl. auto.
+    destruct* (v1 == v).
+  congruence.
+Qed.
+
+Lemma all_size_var : forall v v0 S K pairs,
+  v # S ->
+  all_size (compose (v ~ typ_fvar v0) S) K pairs = all_size S K pairs.
+Proof.
+  unfold all_size; intros.
+  assert (disjoint (dom (v ~ typ_fvar v0)) (dom S)).
+    simpl. intro x; destruct* (x == v).
+  induction pairs; simpl.
+    unfold kinds_size.
+    refine (f_equal (mult _) _).
+    induction (kenv_types K); simpl. auto.
+    rewrite IHl.
+    unfold typ_size'.
+    rewrite* typ_subst_compose.
+    rewrite* typ_size'_var.
+  rewrite plus_assoc.
+  rewrite <- plus_assoc.
+  rewrite IHpairs. clear IHpairs.
+  repeat rewrite* typ_subst_compose.
+  repeat rewrite typ_size'_var.
+  repeat rewrite plus_assoc. auto.
+Qed.
+
+Lemma get_kind_fv_in : forall S v K,
+  kind_fv (kind_subst S (get_kind v K)) << fv_in kind_fv (map (kind_subst S) K).
+Proof.
+  induction K; simpl. apply subset_refl.
+  unfold get_kind; simpl.
+  destruct a. destruct (v == v0).
+    simpl. intros x Hx; auto with sets.
+  fold (get_kind v K).
+  intros x Hx.
+  simpl. apply S.union_3. apply* IHK.
+Qed.
+
+Lemma in_typ_fv : forall t l,
+  In t l -> typ_fv t << typ_fv_list l.
+Proof.
+  induction l; simpl; intros H x Hx. elim H.
+  destruct H.
+    subst; simpl.
+    auto with sets.
+  apply S.union_3; apply* IHl.
+Qed.
+
+Lemma unify_kinds_fv : forall k k0 k1 l S,
+  unify_kinds k k0 = Some (k1, l) ->
+  kind_fv (kind_subst S k1) \u all_fv S l <<
+  kind_fv (kind_subst S k) \u kind_fv (kind_subst S k0).
+Proof.
+  unfold unify_kinds; intros.
+  destruct k as [[kc kv kr kh]|].
+    destruct k0 as [[kc0 kv0 kr0 kh0]|].
+      destruct (cstr_valid (cstr_lub kc kc0)); try discriminate.
+      inversions H; clear H.
+      simpl.
+      unfold kind_fv; simpl.
+      repeat rewrite map_map; simpl.
+      rewrite <- fv_list_map. rewrite <- map_app.
+      set (pairs := nil(A:=typ*typ)).
+      set (kr' := nil(A:=var*typ)).
+      intros x Hx.
+      rewrite <- union_empty_r.
+      replace {} with
+        (typ_fv_list (List.map (fun x : var * typ => typ_subst S (snd x)) kr'))
+        by reflexivity.
+      rewrite <- union_empty_r.
+      replace {} with (all_fv S pairs) by reflexivity.
+      clearbody pairs kr'.
+      gen pairs kr'; induction (kr ++ kr0); simpl; intros.
+        rewrite <- union_assoc; auto with sets.
+      destruct a; simpl in *.
+      destruct (In_dec eq_var_dec v0 (unique (cstr_lub kc kc0))).
+        case_rewrite (get v0 kr') R1;
+          poses Hsub (IHl _ _ Hx); clear IHl.
+          rewrite <- union_assoc in Hsub.
+          destruct (S.union_1 Hsub); clear Hsub; auto with sets.
+          destruct (S.union_1 H); clear H; auto with sets.
+          unfold all_fv in H0; simpl in H0.
+          destruct (S.union_1 H0); clear H0; auto with sets.
+          destruct (S.union_1 H); clear H; auto with sets.
+          use (get_in R1).
+          use (in_map (fun x : var * typ => typ_subst S (snd x)) _ _ H).
+          use (in_typ_fv _ _ H1 H0).
+          auto with sets.
+        simpl in Hsub. union_solve x.
+      poses Hsub (IHl _ _ Hx); clear IHl Hx.
+      simpl in Hsub.
+      union_solve x.
+    inversions H.
+    unfold kind_fv, all_fv; simpl.
+    apply subset_refl.
+  inversions H.
+  unfold kind_fv, all_fv; simpl.
+  rewrite union_comm; apply subset_refl.
+Qed.
+
+Lemma all_fv_app : forall S l1 l2,
+  all_fv S (l1 ++ l2) = all_fv S l1 \u all_fv S l2.
+Proof.
+  intros.
+  unfold all_fv.
+  induction l1; simpl. rewrite* union_empty_l.
+  rewrite IHl1.
+  repeat rewrite union_assoc. auto.
+Qed.
 
 Lemma size_pairs_decr_vars : forall S0 K0 t t0 pairs h v v0 x0 l,
   is_subst S0 -> ok K0 ->
@@ -2341,62 +2177,108 @@ Lemma size_pairs_decr_vars : forall S0 K0 t t0 pairs h v v0 x0 l,
     (remove_env (remove_env K0 v) v0 & v0 ~ x0) (l ++ pairs) < h.
 Proof.
   intros.
-  use (typ_subst_res_fresh _ H H3).
+  use (typ_subst_res_fresh' _ H H3).
+  poses Hv (typ_subst_res_fresh' _ H H2).
   use (typ_subst_disjoint t0 H).
   eapply lt_le_trans; try apply (lt_n_Sm_le _ _ H1).
-  clear H1 H.
+  clear H1.
   unfold size_pairs.
   assert (v \in really_all_fv S0 K0 ((t,t0)::pairs)).
     unfold really_all_fv, all_fv.
     simpl. rewrite H2. simpl; auto with sets.
-  rewrite <- (cardinal_remove H).
+  rewrite <- (cardinal_remove H1). clear H1.
   simpl.
+  set (S := compose (v ~ typ_fvar v0) S0).
   apply pow2exp_lt_le.
-    rewrite all_size_app.
+    eapply le_lt_trans.
+      instantiate (1 := all_size S K0 pairs).
+      destruct (unify_kinds_size _ _ S H5).
+      unfold all_size, kinds_size; simpl.
+      rewrite <- (length_remove_env v K0).
+      repeat rewrite app_length.
+      rewrite <- (length_remove_env v0 (remove_env K0 v)).
+      assert (get_kind v0 (remove_env K0 v) = get_kind v0 K0).
+        unfold get_kind.
+        case_eq (get v0 K0); intros.
+          rewrite* (binds_remove_env (v:=v) H9).
+        case_eq (get v0 (remove_env K0 v)); intros.
+          rewrite (binds_orig_remove_env _ H0 H10) in H9. discriminate.
+        auto.
+      rewrite H9.
+      repeat rewrite app_length.
+      rewrite plus_assoc.
+      rewrite <- (accum_remove_env (typ_size' S) v K0).
+      rewrite all_types_app.
+      repeat rewrite accum_app; try (intros; omega).
+      rewrite <- (accum_remove_env (typ_size' S) v0 (remove_env K0 v)).
+      rewrite accum_app; try (intros; omega).
+      rewrite H9. clear H9.
+      unfold kinds_size in H8.
+      set (K := kenv_types (remove_env (remove_env K0 v) v0)) in *.
+      set (kv := kind_types (get_kind v K0)) in *.
+      set (kv0 := kind_types (get_kind v0 K0)) in *.
+      set (kx0 := kind_types x0) in *.
+      rewrite plus_assoc.
+      replace (accum (typ_size' S) plus 0 kv + accum (typ_size' S) plus 0 kv0)
+        with (accum (typ_size' S) plus 0 (kv ++ kv0))
+        by (rewrite accum_app; intros; omega).
+      replace (length kv + length kv0) with (length (kv ++ kv0))
+        by rewrite* app_length.
+      rewrite mult_plus_distr_r.
+      rewrite mult_plus_distr_r.
+      repeat rewrite plus_assoc.
+      repeat rewrite mult_plus_distr_l.
+      repeat rewrite plus_assoc.
+      apply plus_le_compat_r.
+      use (mult_le_compat_l _ _ (length K) (H1 (typ_size' S))).
+      use (H1 (fun _ => 1)). repeat rewrite <- length_accum in H10.
+      use (mult_le_compat_r _ _ (accum (typ_size' S) plus 0 K) H10).
+      omega.
+    unfold S; clear S.
+    rewrite* all_size_var.
     unfold all_size; simpl.
-    use (typ_subst_decr_all T S K pairs H).
-  assert (typ_size T < all_size S K ((typ_fvar v, T) :: pairs)).
-    unfold all_size; simpl.
-    rewrite* get_notin_dom.
-    rewrite (typ_subst_fresh S T); try disjoint_solve.
-    simpl; omega.
-  assert (all_size S K pairs < all_size S K ((typ_fvar v, T) :: pairs)).
-    unfold all_size; simpl.
-    rewrite* get_notin_dom.
-    simpl; omega.
-  eapply le_lt_trans. apply all_size_remove.
-  eapply le_lt_trans. apply H3.
-  rewrite mult_comm.
-  eapply le_lt_trans; try (eapply mult_lt_compat_r; try apply H5).
-    apply mult_le_compat_l. omega.
-  destruct T; simpl; omega.
-
-
-
-  assert (S.cardinal (really_all_fv (compose (v ~ typ_fvar v0) S0)
-           (remove_env (remove_env K0 v) v0 & v0 ~ x0) 
-           (l ++ pairs) <<
-  unfold really_all_fv.
-  rewrite all_fv_app.
-  assert (
-  poses Hfv (unify_kinds_fv _ _ S0 H5).
+    set (T := typ_subst S0 t).
+    assert (typ_size T > 0). destruct T; simpl; omega.
+    destruct (typ_size T). omega.
+    simpl.
+    repeat rewrite <- plus_assoc.
+    apply le_lt_n_Sm.
+    eapply le_trans; [|apply le_plus_r].
+    eapply le_trans; [|apply le_plus_r].
+    rewrite plus_assoc. apply le_plus_l.
+  poses Hfv (unify_kinds_fv _ _ S H5).
+  apply cardinal_subset.
+  intros x Hx.
+  replace (really_all_fv S0 K0 ((t, t0) :: pairs))
+    with (really_all_fv S0 K0 ((typ_fvar v, typ_fvar v0) :: pairs)).
+    apply* really_all_fv_decr.
+      simpl; intro y; destruct* (y == v0). subst*.
+    fold S.
+    unfold really_all_fv in *.
+    simpl in *.
+    rewrite all_fv_app in Hx.
+    destruct (S.union_1 Hx); clear Hx.
+      destruct (S.union_1 H1); clear H1.
+      use (Hfv x (S.union_2 _ H8)).
+      clear -H1.
+      apply S.union_2.
+      destruct (S.union_1 H1); apply (get_kind_fv_in _ _ _ H).
+      rewrite map_remove_env in H8.
+      use (fv_in_remove_env _ _ _ H8).
+      rewrite map_remove_env in H1.
+      apply S.union_2.
+      use (fv_in_remove_env _ _ _ H1).
+    destruct (S.union_1 H1); clear H1.
+      apply S.union_2.
+      use (Hfv _ (S.union_3 _ H8)).
+      clear -H1.
+      destruct (S.union_1 H1); apply (get_kind_fv_in _ _ _ H).
+    auto with sets.
+  unfold really_all_fv, all_fv.
+  rewrite <- H2; rewrite <- H3.
   simpl.
-    apply size_pairs_decr.
-    assert (disjoint {{v}} (typ_fv (typ_subst S0 t0))).
-      intro v0. destruct* (v0 == v).
-      subst.
-      right; intro.
-      rewrite (S.mem_1 H6) in H1. discriminate.
-    disjoint_solve.
-  replace (size_pairs S0 K0 ((typ_fvar v, typ_subst S0 t0) :: pairs))
-    with (size_pairs S0 K0 ((t, t0) :: pairs)).
-    omega.
-  unfold size_pairs, all_size, really_all_fv, all_fv; simpl.
-  rewrite* get_notin_dom.
-  rewrite H3.
-  rewrite* typ_subst_idem.
+  repeat rewrite* typ_subst_idem.
 Qed.
-  
 
 Lemma typ_subst_eq_add : forall S S0 v T T1 T2 pairs,
   (forall T1 T2 : typ,
@@ -2449,6 +2331,14 @@ Section Completeness.
 
 Variables (K:kenv) (S:subs).
 
+Definition complete_spec S0 K0 pairs h :=
+  is_subst S0 -> ok K0 ->
+  (forall T, typ_subst S (typ_subst S0 T) = typ_subst S T) ->
+  (forall T1 T2, In (T1, T2) pairs -> typ_subst S T1 = typ_subst S T2) ->
+  well_subst K0 K S ->
+  size_pairs S0 K0 pairs < h ->
+  unify h pairs K0 S0 <> None.
+
 Lemma unify_complete_nv : forall pairs K0 S0 v T h t t0,
   typ_subst S0 t = typ_fvar v ->
   typ_subst S0 t0 = T ->
@@ -2495,14 +2385,9 @@ Proof.
   rewrite <- R2 in H.
   use (size_pairs_decr' _ _ _ HS0 HK0 H Hsz R1).
   rewrite R2 in H2.
-  use (typ_subst_res_fresh _ HS0 R1).
+  use (typ_subst_res_fresh' _ HS0 R1).
+  rewrite R2 in H.
   revert H1; apply* IHh; clear IHh.
-      apply* add_binding_is_subst.
-      use (typ_subst_disjoint t0 HS0).
-      rewrite R2 in *; simpl in *.
-      assert (disjoint {{v}} (typ_fv T)).
-        intro x; destruct (x == v); subst; auto.
-      disjoint_solve.
     intros. rewrite* typ_subst_compose.
     rewrite typ_subst_prebind. apply Hext. congruence.
     simpl; intro x; destruct* (x == v).
@@ -2514,6 +2399,108 @@ Proof.
     rewrite* dom_remove_env. apply* S.remove_1.
   apply WS.
   apply* binds_orig_remove_env.
+Qed.
+
+Lemma well_kinded_kind_entails: forall K k x,
+  well_kinded K k (typ_fvar x) -> kind_entails (get_kind x K) k.
+Proof.
+  intros; unfold kind_entails.
+  inversions H. auto.
+  rewrite* (binds_get_kind H1).
+Qed.
+
+Lemma unify_complete_vars : forall h t t0 pairs K0 S0 v v0,
+  is_subst S0 -> ok K0 ->
+  (forall T : typ, typ_subst S (typ_subst S0 T) = typ_subst S T) ->
+  (forall T1 T2 : typ,
+    In (T1, T2) ((t, t0) :: pairs) -> typ_subst S T1 = typ_subst S T2) ->
+  well_subst K0 K S ->
+  size_pairs S0 K0 ((t, t0) :: pairs) < Datatypes.S h ->
+  typ_subst S0 t = typ_fvar v ->
+  typ_subst S0 t0 = typ_fvar v0 ->
+  v <> v0 ->
+  (forall pairs K0 S0, is_subst S0 -> ok K0 ->
+    (forall T : typ, typ_subst S (typ_subst S0 T) = typ_subst S T) ->
+    (forall T1 T2 : typ,
+      In (T1, T2) pairs -> typ_subst S T1 = typ_subst S T2) ->
+    well_subst K0 K S ->
+    size_pairs S0 K0 pairs < h -> unify h pairs K0 S0 <> None) ->
+  match unify_vars K0 v v0 with
+  | Some (pair K' pairs0) =>
+    unify h (pairs0 ++ pairs) K' (compose (v ~ typ_fvar v0) S0)
+  | None => None (A:=kenv * subs)
+  end <> None.
+Proof.
+  intros until v0; intros HS0 HK0 Hext Heq WS Hsz R1 R2 n IHh.
+  unfold unify_vars.
+  poses Hv (typ_subst_res_fresh' _ HS0 R1).
+  poses Wk (well_subst_get_kind v WS).
+  poses Wk0 (well_subst_get_kind v0 WS).
+  set (S0' := compose (v ~ typ_fvar v0) S0) in *.
+  assert (HS0': is_subst S0') by (unfold S0'; auto*).
+  assert (HK0': forall y, ok (remove_env (remove_env K0 v) v0 & v0 ~ y)).
+    use (ok_remove_env v HK0).
+    constructor. apply* ok_remove_env.
+    rewrite* dom_remove_env. apply S.remove_1. reflexivity.
+  assert (Hext': forall T, typ_subst S (typ_subst S0' T) = typ_subst S T).
+    intros. unfold S0'. rewrite* typ_subst_compose.
+    rewrite typ_subst_prebind. apply Hext.
+    rewrite <- R1; rewrite <- R2.
+    symmetry; repeat rewrite Hext; apply* Heq.
+    clear -Hv; simpl; intro y; destruct* (y == v).
+  assert (Sv_Sv0 : typ_subst S (typ_fvar v) = typ_subst S (typ_fvar v0)).
+    rewrite <- R1; rewrite <- R2.
+    repeat rewrite Hext. apply* Heq.
+  assert (get_kind v K0 = None /\ get_kind v0 K0 = None \/
+        exists v1, typ_subst S (typ_fvar v0) = typ_fvar v1
+          /\ kind_entails (get_kind v1 K) (kind_subst S (get_kind v K0))
+          /\ kind_entails (get_kind v1 K) (kind_subst S (get_kind v0 K0))).
+    case_rewrite (get_kind v0 K0) R3.
+      inversions Wk0. right; exists x. rewrite H0; split*.
+      simpl in Wk0; rewrite <- H0 in Wk0.
+      rewrite Sv_Sv0 in Wk; simpl in Wk; rewrite <- H0 in Wk.
+      split; apply* well_kinded_kind_entails.
+    case_rewrite (get_kind v K0) R4.
+      inversions Wk. right; exists x.
+      rewrite <- Sv_Sv0; rewrite H0.
+      split*.
+      split; apply well_kinded_kind_entails.
+      rewrite* H0.
+      apply wk_any.
+    left*.
+  destruct H as [[G G0]|[v1 [Hv1 [KEv KEv0]]]].
+    rewrite G; rewrite G0.
+    simpl unify_kinds. lazy iota beta.
+    apply* IHh.
+      intro; intros.
+      binds_cases H.
+        use (binds_orig_remove_env _ (ok_remove_env v HK0) B).
+        destruct (Z == v).
+          subst. elim (binds_fresh H).
+          rewrite dom_remove_env. apply S.remove_1. reflexivity. auto.
+        use (binds_orig_remove_env _ HK0 H).
+      subst. apply wk_any.
+    unfold S0'; apply* size_pairs_decr_vars.
+    rewrite G; rewrite G0; reflexivity.
+  destruct (unify_kinds_complete _ _ _ _ KEv KEv0)
+    as [k1 [l [HU [Heql KEk1]]]].
+  rewrite HU.
+  apply* IHh.
+      intros. destruct* (in_app_or _ _ _ H).
+    intro; intros.
+    binds_cases H.
+      apply WS.
+      apply* binds_orig_remove_env.
+      apply* binds_orig_remove_env.
+    subst.
+    rewrite Hv1.
+    case_rewrite (get_kind v1 K) R3.
+      destruct k1; simpl in *; auto.
+        eapply wk_kind. apply (get_kind_binds _ _ R3). auto.
+      apply wk_any.
+    destruct (kind_subst S k1); simpl in KEk1. elim KEk1.
+    apply wk_any.
+  unfold S0'; apply* size_pairs_decr_vars.
 Qed.
 
 Lemma unify_complete0 : forall h pairs K0 S0,
@@ -2557,104 +2544,34 @@ Proof.
        subst.
        apply* (IHh pairs K0 S0 HS0).
        use (size_pairs_grows S0 K0 (t,t0) pairs). omega.
-      unfold unify_vars.
-      poses Hv (typ_subst_res_fresh _ HS0 R1).
-      poses Wk (well_subst_get_kind v WS).
-      poses Wk0 (well_subst_get_kind v0 WS).
-      case_rewrite (get_kind v0 K0) R3.
-        simpl in Wk0; inversions Wk0; clear Wk0.
-        destruct (unify_kinds_complete (get_kind v K0) (get_kind v0 K0)
-                  (get_kind x K) S); unfold kind_entails.
-          rewrite (binds_get_kind H2).
-          case_rewrite (get_kind v K0) R4.
-           assert (typ_subst S (typ_fvar v) = typ_fvar x).
-             rewrite H0.
-             fold (typ_subst S (typ_fvar v0)).
-             rewrite <- R1; rewrite <- R2.
-             repeat rewrite Hext; apply* Heq.
-           rewrite H in Wk.
-           simpl in Wk; inversions Wk; clear Wk.
-           use (binds_func H6 H2).
-           inversions H1; clear H1 H6.
-           simpl*.
-          simpl*.
-         rewrite R3.
-         rewrite (binds_get_kind H2).
-         simpl*.
-        destruct H as [l [UK [FA KE]]].
-        rewrite <- R3; rewrite UK.
-        apply* IHh.
-             apply* add_binding_is_subst.
-             use (typ_subst_disjoint t0 HS0).
-             rewrite R2 in *; simpl in *.
-             intro. destruct* (x1 == v0). subst; destruct* (H v0).
-            use (ok_remove_env v HK0).
-            constructor. apply* ok_remove_env.
-            rewrite* dom_remove_env. apply S.remove_1. reflexivity.
-           intros. rewrite* typ_subst_compose.
-           rewrite typ_subst_prebind. apply Hext.
-           rewrite <- R1; rewrite <- R2.
-           symmetry; repeat rewrite Hext; apply* Heq.
-           clear -Hv; simpl; intro y; destruct* (y == v).
-          intros. destruct* (in_app_or _ _ _ H).
-         intro; intros.
-         binds_cases H.
-           apply WS.
-           apply* binds_orig_remove_env.
-           apply* binds_orig_remove_env.
-         destruct (binds_single_inv B0); subst.
-         clear B0 H H4.
-         apply* kind_entails_well_kinded.
-         rewrite (binds_get_kind H2).
-         simpl; rewrite <- H0.
-         apply* wk_kind. apply entails_refl.
-           
-       case_rewrite (get_kind v0 K0) R.
-        simpl in Wk; inversions Wk; clear Wk.
-        destruct (unify_kinds_complete (get_kind v K0) (get_kind v0 K0)
-                  (get_kind x K) S); unfold kind_entails.
-          rewrite (binds_get_kind H2). rewrite R3.
-          simpl*.
-
-        use (well_subst_get_kind v WS).
-        inversions H.
-          destruct (get_kind v0); simpl*.
-        rewrite H0.
-        
-      case_eq (unify_kinds (get_kind v K0) (get_kind v0 K0)); introv R3.
-
-      destruct* (unify_complete_step S R1 R2 Hsz).
-      intro; elim n. inversions* H.
-     destruct* (unify_complete_step S R1 R2 Hsz).
-      intro; discriminate.
-     rewrite* H.
-    assert (In (t,t0) ((t,t0)::pairs)) by simpl*.
-    use (Heq _ _ H); clear H.
-    rewrite R1 in H0; rewrite R2 in H0.
+      apply* unify_complete_vars.
+     apply* unify_complete_nv.
+     intro; discriminate.
+    assert (In (t,t0) ((t,t0)::pairs)) by auto.
+    poses E (Heq _ _ H).
+    rewrite <- (Hext t) in E. rewrite R1 in E.
+    rewrite <- (Hext t0) in E. rewrite R2 in E.
     discriminate.
    rewrite size_pairs_comm in Hsz.
-   destruct* (unify_complete_step S R2 R1 Hsz).
+   apply* unify_complete_nv.
      simpl; intros. destruct H; subst.
        inversions H; symmetry; apply* Heq.
      apply* Heq.
-    intro; discriminate.
-   rewrite* H.
-  destruct* (IHh ((t1,t3)::(t2,t4)::pairs) S0 S); clear IHh.
-    clear Hsz; intros.
-    assert (In (t,t0) ((t,t0)::pairs)) by simpl*.
+   intro; discriminate.
+  apply* IHh.
+    clear IHh Hsz; intros.
+    assert (In (t,t0) ((t,t0)::pairs)) by auto.
     use (Heq _ _ H0).
-    rewrite <- (typ_subst_idem t HS0) in H1.
-    rewrite <- (typ_subst_idem t0 HS0) in H1.
+    rewrite <- (Hext t) in H1.
+    rewrite <- (Hext t0) in H1.
     rewrite R1 in H1; rewrite R2 in H1.
-    simpl in H1; inversions H1; clear H1.
-    simpl in H; destruct H.
-      inversions* H.
-    simpl in H; destruct H.
-      inversions* H.
+    simpl in H1; inversions H1.
+    simpl in H; destruct H. inversions* H.
+    destruct H. inversions* H.
     apply* Heq.
-  assert (size_pairs S0 ((t1, t3) :: (t2, t4) :: pairs) <
-          size_pairs S0 ((t, t0) :: pairs)).
-    unfold size_pairs, all_size, all_fv.
+  assert (size_pairs S0 K0 ((t1, t3) :: (t2, t4) :: pairs) <
+          size_pairs S0 K0 ((t, t0) :: pairs)).
+    unfold size_pairs, all_size, really_all_fv, all_fv.
     simpl.
     rewrite <- (typ_subst_idem t HS0).
     rewrite <- (typ_subst_idem t0 HS0).
@@ -2668,17 +2585,19 @@ Proof.
   omega.
 Qed.
 
-Theorem unify_complete : forall T1 T2 S,
+Theorem unify_complete : forall T1 T2 K0,
+  ok K0 -> well_subst K0 K S ->
   typ_subst S T1 = typ_subst S T2 ->
-  exists S',
-    unify ((T1,T2)::nil) id (1 + size_pairs id ((T1,T2)::nil)) = Some S'.
+  unify (1 + size_pairs id K0 ((T1,T2)::nil)) ((T1,T2)::nil) K0 id <> None.
 Proof.
   intros.
   apply* unify_complete0.
-    apply is_subst_id.
-  intros. rewrite (typ_subst_id T0). rewrite (typ_subst_id T3).
-  simpl in H0; destruct* H0.
-  inversions* H0.
+      apply is_subst_id.
+    intros; rewrite* typ_subst_id.
+  intros; simpl in H2; destruct* H2.
+  inversions* H2.
 Qed.
+
+End Completeness.
 
 End MkInfer.
